History independence removed and equivalence lemmas reworked to not require history independence. Currently, equivalence lemmas for read and write are commented out (other files need to be updated with new operational semantics first) and equivalence lemma for shifted variables is commented out (stuck on the proof).

rupicola/io/ExpRel.fst
@@ -145,6 +145,14 @@ let lem_forall_values_are_values t h fs_e :
     end
   end
 
+let lem_forall_values_are_values_prod t h :
+  Lemma (forall (e:closed_exp) (lt:local_trace h) (fs_r:get_Type t). t ∋ (h++lt, fs_r, e) ==> is_value e) = 
+  introduce forall e lt fs_r. t ∋ (h++lt, fs_r, e) ==> is_value e with begin
+    introduce _ ==> _ with _. begin
+      lem_values_are_values t (h++lt) fs_r e
+    end
+  end
+
 (** F* Evaluation Environment : variable -> value **)
 
 (** We compile F* values, not F* expressions.
@@ -608,7 +616,7 @@ let equiv_pair #g
     end
   end
 
-(*let equiv_pair_fst_app #g
+let equiv_pair_fst_app #g
   (#t1 #t2:qType)
   (fs_e12:fs_oval g (t1 ^* t2))
   (e12:exp)
@@ -627,12 +635,9 @@ let equiv_pair #g
         introduce steps e e' h lt /\ indexed_irred e' (h++lt) ==> (t1 ∋ (h, fs_e, e') /\ lt == []) with _. begin
           let steps_e_e' : squash (steps e e' h lt) = () in
           FStar.Squash.map_squash #_ #(squash (t1 ∋ (h, fs_e, e') /\ lt == [])) steps_e_e' (fun steps_e_e' ->
-            exp_type_history_independence (t1 ^* t2) h fs_e12 e12;
-            safety_val #(t1 ^* t2) fs_e12 e12;
-            sem_expr_shape_val #(t1 ^* t2) fs_e12 e12 h;
-            let t1_typ = type_quotation_to_typ (get_rel t1) in
-            let t2_typ = type_quotation_to_typ (get_rel t2) in
-            let (e12', (| lt12, lt_f |)) = destruct_steps_epair_fst e12 e' h lt steps_e_e' t1_typ t2_typ in
+            lem_forall_values_are_values (t1 ^* t2) h fs_e12;
+            assert (forall e12' lt12. (steps e12 e12' h lt12 /\ indexed_irred e12' (h++lt12)) ==> (EPair? e12' /\ is_value e12'));
+            let (e12', (| lt12, lt_f |)) = destruct_steps_epair_fst e12 e' h lt steps_e_e' in
             lem_value_is_irred e12';
             assert ((t1 ^* t2) ⦂ (h, fs_e12, e12));
             eliminate forall e12' lt12. steps e12 e12' h lt12 /\ indexed_irred e12' (h++lt12) ==> ((t1 ^* t2) ∋ (h, fs_e12, e12') /\ lt12 == []) with e12' lt12;
@@ -664,12 +669,9 @@ let equiv_pair_snd_app #g (#t1 #t2:qType) (fs_e12:fs_oval g (t1 ^* t2)) (e12:exp
         introduce steps e e' h lt /\ indexed_irred e' (h++lt) ==> (t2 ∋ (h, fs_e, e') /\ lt == []) with _. begin
           let steps_e_e' : squash (steps e e' h lt) = () in
           FStar.Squash.map_squash #_ #(squash (t2 ∋ (h, fs_e, e') /\ lt == [])) steps_e_e' (fun steps_e_e' ->
-            exp_type_history_independence (t1 ^* t2) h fs_e12 e12;
-            safety_val #(t1 ^* t2) fs_e12 e12;
-            sem_expr_shape_val #(t1 ^* t2) fs_e12 e12 h;
-            let t1_typ = type_quotation_to_typ (get_rel t1) in
-            let t2_typ = type_quotation_to_typ (get_rel t2) in
-            let (e12', (| lt12, lt_f |)) = destruct_steps_epair_snd e12 e' h lt steps_e_e' t1_typ t2_typ in
+            lem_forall_values_are_values (t1 ^* t2) h fs_e12;
+            assert (forall e12' lt12. (steps e12 e12' h lt12 /\ indexed_irred e12' (h++lt12)) ==> (EPair? e12' /\ is_value e12'));
+            let (e12', (| lt12, lt_f |)) = destruct_steps_epair_snd e12 e' h lt steps_e_e' in
             lem_value_is_irred e12';
             assert ((t1 ^* t2) ⦂ (h, fs_e12, e12));
             eliminate forall e12' lt12. steps e12 e12' h lt12 /\ indexed_irred e12' (h++lt12) ==> ((t1 ^* t2) ∋ (h, fs_e12, e12') /\ lt12 == []) with e12' lt12;
@@ -701,15 +703,13 @@ let equiv_inl #g (#t1 t2:qType) (fs_e:fs_oval g t1) (e:exp) : Lemma
         introduce _ ==> (t ∋ (h, fs_ex, ex') /\ lt == []) with _. begin
           let steps_e_e' : squash (steps ex ex' h lt) = () in
           FStar.Squash.map_squash #_ #(squash (t ∋ (h, fs_ex, ex') /\ lt == [])) steps_e_e' (fun steps_e_e' ->
-            exp_type_history_independence t1 h fs_e e;
-            safety_val #t1 fs_e e;
-            let t1_typ = type_quotation_to_typ (get_rel t1) in
-            let t2_typ = type_quotation_to_typ (get_rel t2) in
-            let (e', (| lt12, lt_f |)) = destruct_steps_einl e ex' h lt steps_e_e' t1_typ t2_typ in
+            lem_forall_values_are_values t1 h fs_e;
+            assert (forall e' lt'. steps e e' h lt' /\ indexed_irred e' (h++lt') ==> is_value e');
+            let (e', (| lt12, lt_f |)) = destruct_steps_einl e ex' h lt steps_e_e' in
             lem_value_is_irred e';
             lem_value_is_irred (EInl e');
             assert (t1 ∋ (h, fs_e, e') /\ lt12 == []);
-            lem_destruct_steps_einl e' ex' h lt_f t1_typ t2_typ;
+            lem_destruct_steps_einl e' ex' h lt_f;
             assert (t ∋ (h, fs_ex, ex'))
           )
         end
@@ -733,15 +733,13 @@ let equiv_inr #g (t1 #t2:qType) (fs_e:fs_oval g t2) (e:exp) : Lemma
         introduce _ ==> (t ∋ (h, fs_ex, ex') /\ lt == []) with _. begin
           let steps_e_e' : squash (steps ex ex' h lt) = () in
           FStar.Squash.map_squash #_ #(squash (t ∋ (h, fs_ex, ex') /\ lt == [])) steps_e_e' (fun steps_e_e' ->
-            exp_type_history_independence t2 h fs_e e;
-            safety_val #t2 fs_e e;
-            let t1_typ = type_quotation_to_typ (get_rel t1) in
-            let t2_typ = type_quotation_to_typ (get_rel t2) in
-            let (e', (| lt12, lt_f |)) = destruct_steps_einr e ex' h lt steps_e_e' t1_typ t2_typ in
+            lem_forall_values_are_values t2 h fs_e;
+            assert (forall e' lt'. steps e e' h lt' /\ indexed_irred e' (h++lt') ==> is_value e');
+            let (e', (| lt12, lt_f |)) = destruct_steps_einr e ex' h lt steps_e_e' in
             lem_value_is_irred e';
             lem_value_is_irred (EInr e');
             assert (t2 ∋ (h, fs_e, e') /\ lt12 == []);
-            lem_destruct_steps_einr e' ex' h lt_f t1_typ t2_typ;
+            lem_destruct_steps_einr e' ex' h lt_f;
             assert (t ∋ (h, fs_ex, ex'))
           )
         end
@@ -761,13 +759,10 @@ let equiv_case_steps_pre (e e':closed_exp) (h:history) (lt:local_trace h) (t1 t2
   ((t2 ^-> t3) ⦂ (h, fs_rc_lam, ELam e_rc))
 
 let equiv_case_steps #e #e' #h #lt #t1 #t2 #t3 #fs_case #fs_lc_lam #fs_rc_lam #fs_e #e_case #e_lc #e_rc (sq:squash (equiv_case_steps_pre e e' h lt t1 t2 t3 fs_case fs_lc_lam fs_rc_lam fs_e e_case e_lc e_rc)) : squash (t3 ∋ (h, fs_e, e') /\ lt == []) =
-  exp_type_history_independence (t1 ^+ t2) h fs_case e_case;
-  safety_val #(t1 ^+ t2) fs_case e_case;
-  sem_expr_shape_val #(t1 ^+ t2) fs_case e_case h;
-  let t1_typ = type_quotation_to_typ (get_rel t1) in
-  let t2_typ = type_quotation_to_typ (get_rel t2) in
+  lem_forall_values_are_values (t1 ^+ t2) h fs_case;
+  assert (forall e_case' lt'. steps e_case e_case' h lt' /\ indexed_irred e_case' (h++lt') ==> ((EInl? e_case' \/ EInr? e_case') /\ is_value e_case'));
   FStar.Squash.bind_squash #(steps e e' h lt) () (fun sts ->
-    let (e_case', (| lt1, (lt2, lt3) |)) = destruct_steps_ecase e_case e_lc e_rc e' h lt sts t1_typ t2_typ in
+    let (e_case', (| lt1, (lt2, lt3) |)) = destruct_steps_ecase e_case e_lc e_rc e' h lt sts in
     match e_case' with
     | EInl e_c' -> begin
       assert (steps (ELam e_lc) (ELam e_lc) h []);
@@ -835,7 +830,7 @@ let equiv_case
       end
     end
   end
-#pop-options*)
+#pop-options
 
 let equiv_lam_prod #g (#t1:qType) (#t2:qType) (fs_body:fs_oprod (extend t1 g) t2) (body:exp)
   : Lemma
@@ -1007,21 +1002,14 @@ let equiv_bind_steps_pre (e e':closed_exp) (h:history) (lt:local_trace h) (a:qTy
   (forall (lt:local_trace h). ((a ^->!@ b) ⦂ (h++lt, fs_k', (ELam k'))))
 
 let equiv_bind_steps #e #e' #h #lt #a #b #fs_k' #fs_m #fs_e' #m #k' (sq:squash (equiv_bind_steps_pre e e' h lt a b fs_k' fs_m fs_e' m k')) : squash (exists (fs_r:get_Type b). b ∋ (h++lt, fs_r, e') /\ fs_beh fs_e' h lt fs_r) =
-  assert (a ⪾ (h, fs_m, m));
-  assert (forall m' lt2. steps m m' h lt2 /\ indexed_irred m' (h++lt2) ==> (exists (fs_r:get_Type a). a ∋ (h++lt2, fs_r, m') /\ fs_beh fs_m h lt2 fs_r));
-  assume (forall m' (fs_r:get_Type a) lt2. a ∋ (h++lt2, fs_r, m') ==> is_value m');
+  lem_forall_values_are_values_prod a h; 
   assert (forall m' lt2. steps m m' h lt2 /\ indexed_irred m' (h++lt2) ==> is_value m');
-  let a_typ = type_quotation_to_typ (get_rel a) in
-  let b_typ = type_quotation_to_typ (get_rel b) in
   FStar.Squash.bind_squash #(steps e e' h lt) () (fun sts ->
-  let (m', (| lt2, lt' |)) = destruct_steps_eapp_e2 (ELam k') m e' h lt sts a_typ b_typ in
-  assert (lt == (lt2 @ lt'));
+  let (m', (| lt2, lt' |)) = destruct_steps_eapp_e2 (ELam k') m e' h lt sts in
   assert ((a ^->!@ b) ⦂ (h++lt2, fs_k', (ELam k')));
   assert (forall k_ (lt1:local_trace (h++lt2)). (steps (ELam k') k_ (h++lt2) lt1 /\ indexed_irred k_ ((h++lt2)++lt1)) ==> (ELam? k_ /\ is_closed k_));
   FStar.Squash.bind_squash #(steps (EApp (ELam k') m') e' (h++lt2) lt') () (fun sts2 ->
-  let (k1, (| lt1, lt'' |)) = destruct_steps_eapp_e1 (ELam k') m' e' (h++lt2) lt' sts2 a_typ b_typ in
-  assert (lt' == (lt1 @ lt''));
-  assert (lt == (lt2 @ (lt1 @ lt'')));
+  let (k1, (| lt1, lt'' |)) = destruct_steps_eapp_e1 (ELam k') m' e' (h++lt2) lt' sts2 in
   lem_value_is_irred m';
   eliminate forall lt2 m'. steps m m' h lt2 /\ indexed_irred m' (h++lt2) ==> (exists (fs_r_m:get_Type a). a ∋ (h++lt2, fs_r_m, m') /\ fs_beh fs_m h lt2 fs_r_m) with lt2 m';
   lem_value_is_irred (ELam k1);
@@ -1029,11 +1017,6 @@ let equiv_bind_steps #e #e' #h #lt #a #b #fs_k' #fs_m #fs_e' #m #k' (sq:squash (
   unroll_elam_io a b (h++lt2) fs_k' k1;
   eliminate exists (fs_r_m:get_Type a). a ∋ (h++lt2, fs_r_m, m') /\ fs_beh fs_m h lt2 fs_r_m
   returns exists (fs_r:get_Type b). b ∋ (h++lt, fs_r, e') /\ fs_beh fs_e' h lt fs_r with _. begin
-  assert (a ∋ (h++lt2, fs_r_m, m'));
-  assert (b ⪾ (h++lt2, fs_k' fs_r_m, subst_beta m' k1));
-  assert (forall lt e'. steps (subst_beta m' k1) e' (h++lt2) lt /\ indexed_irred e' ((h++lt2)++lt) ==> (exists (fs_r':get_Type b). b ∋ ((h++lt2)++lt, fs_r', e') /\ fs_beh (fs_k' fs_r_m) (h++lt2) lt fs_r'));
-  assert (steps (subst_beta m' k1) e' (h++lt2) lt'');
-  assert (indexed_irred e' ((h++lt2)++lt''));
   eliminate exists (fs_r':get_Type b). b ∋ ((h++lt2)++lt'', fs_r', e') /\ fs_beh (fs_k' fs_r_m) (h++lt2) lt'' fs_r'
   returns exists (fs_r:get_Type b). b ∋ (h++lt, fs_r, e') /\ fs_beh fs_e' h lt fs_r with _. begin
   lem_theta_bind #(get_Type a) #(get_Type b) fs_m h lt2 fs_r_m fs_k' lt'' fs_r' lt
@@ -1088,29 +1071,16 @@ let equiv_oprod_app #g (#a #b:qType) (fs_f:fs_oval g (a ^->!@ b)) (fs_x:fs_oval 
         introduce _ ==> (exists (fs_r:get_Type b). b ∋ (h++lt, fs_r, e') /\ fs_beh fs_e h lt fs_r) with _. begin
           let steps_e_e' : squash (steps e e' h lt) = () in
           FStar.Squash.map_squash #_ #(squash (exists (fs_r:get_Type b). b ∋ (h++lt, fs_r, e') /\ fs_beh fs_e h lt fs_r)) steps_e_e' (fun steps_e_e' ->
-            (*exp_type_history_independence a h fs_x x;
-            exp_type_history_independence (a ^->!@ b) h fs_f f;
-            safety_val #a fs_x x;
-            safety_val #(a ^->!@ b) fs_f f;
-            sem_expr_shape_val #(a ^->!@ b) fs_f f h;
-            let a_typ = type_quotation_to_typ (get_rel a) in
-            let b_typ = type_quotation_to_typ (get_rel b) in
-            let (f1, x', (| lt2, (| lt1, lt3 |) |)) = destruct_steps_eapp f x e' h lt steps_e_e' a_typ b_typ in*)
-            assume (forall x' lt2. steps x x' h lt2 /\ indexed_irred x' (h++lt2) ==> is_value x');
-            let a_typ = type_quotation_to_typ (get_rel a) in
-            let b_typ = type_quotation_to_typ (get_rel b) in
-            let (x', (| lt2, lt' |)) = destruct_steps_eapp_e2 f x e' h lt steps_e_e' a_typ b_typ in
+            lem_forall_values_are_values a h fs_x;
+            let (x', (| lt2, lt' |)) = destruct_steps_eapp_e2 f x e' h lt steps_e_e' in
             lem_shift_type_value_environments h fsG s;
             assert (forall f' (lt1:local_trace (h++lt2)). (steps f f' (h++lt2) lt1 /\ indexed_irred f' ((h++lt2)++lt1)) ==> (ELam? f' /\ is_closed f'));
             FStar.Squash.bind_squash #(steps (EApp f x') e' (h++lt2) lt') () (fun sts2 ->
-            let (f1, (| lt1, lt'' |)) = destruct_steps_eapp_e1 f x' e' (h++lt2) lt' sts2 a_typ b_typ in
-            assert (a ⦂ (h, fs_x, x));
-            assert (forall x' lt2. steps x x' h lt2 /\ indexed_irred x' (h++lt2) ==> (a ∋ (h, fs_x, x') /\ lt2 == []));
+            let (f1, (| lt1, lt'' |)) = destruct_steps_eapp_e1 f x' e' (h++lt2) lt' sts2 in
+            eliminate forall x' lt2. steps x x' h lt2 /\ indexed_irred x' (h++lt2) ==> (a ∋ (h, fs_x, x') /\ lt2 == []) with x' lt2;
             lem_value_is_irred x';
-            assert (a ∋ (h, fs_x, x') /\ lt2 == []);
             eliminate forall f' lt1. steps f f' h lt1 /\ indexed_irred f' (h++lt1) ==> ((a ^->!@ b) ∋ (h, fs_f, f') /\ lt1 == []) with (ELam f1) lt1;
             lem_value_is_irred (ELam f1);
-            assert ((a ^->!@ b) ∋ (h, fs_f, (ELam f1)) /\ lt1 == []);
             unroll_elam_io a b h fs_f f1;
             assert (b ⪾ (h, fs_e, subst_beta x' f1));
             assert (exists (fs_r:get_Type b). b ∋ (h++lt, fs_r, e') /\ fs_beh fs_e h lt fs_r)))
@@ -1119,7 +1089,7 @@ let equiv_oprod_app #g (#a #b:qType) (fs_f:fs_oval g (a ^->!@ b)) (fs_x:fs_oval 
     end
   end
 
-(*let equiv_if_prod_steps_pre (ex ex':closed_exp) (h:history) (lt:local_trace h) (a:qType) (fs_c:bool) (fs_t fs_e fs_ex:fs_prod a) (c t e:closed_exp) =
+let equiv_if_prod_steps_pre (ex ex':closed_exp) (h:history) (lt:local_trace h) (a:qType) (fs_c:bool) (fs_t fs_e fs_ex:fs_prod a) (c t e:closed_exp) =
   (fs_ex == (if fs_c then fs_t else fs_e)) /\
   (ex == (EIf c t e)) /\
   (steps ex ex' h lt) /\
@@ -1129,20 +1099,16 @@ let equiv_oprod_app #g (#a #b:qType) (fs_f:fs_oval g (a ^->!@ b)) (fs_x:fs_oval 
   (a ⪾ (h, fs_e, e))
 
 let equiv_if_prod_steps #ex #ex' #h #lt #a #fs_c #fs_t #fs_e #fs_ex #c #t #e (sq:squash (equiv_if_prod_steps_pre ex ex' h lt a fs_c fs_t fs_e fs_ex c t e)) : squash (exists (fs_r:get_Type a). a ∋ (h++lt, fs_r, ex') /\ fs_beh fs_ex h lt fs_r) =
-  exp_type_history_independence qBool h fs_c c;
-  io_exp_type_history_independence a h fs_t t;
-  io_exp_type_history_independence a h fs_e e;
-  safety_val #qBool fs_c c;
-  sem_expr_shape_val #qBool fs_c c h;
+  assert (forall c' lt'. (steps c c' h lt' /\ indexed_irred c' (h++lt')) ==> (ETrue? c' \/ EFalse? c'));
   FStar.Squash.bind_squash #(steps ex ex' h lt) () (fun sts ->
-    let (c', (| lt1, (lt2, lt3) |)) = destruct_steps_eif c t e ex' h lt sts in
-    assert (qBool ∋ (h, fs_c, c') /\ lt1 == []);
-    introduce ETrue? c' ==> (exists (fs_r:get_Type a). a ∋ (h++lt, fs_r, ex') /\ fs_beh fs_ex h lt fs_r) with _. begin
-      assert (exists (fs_r:get_Type a). a ∋ (h++lt2, fs_r, ex') /\ fs_beh fs_t h lt2 fs_r)
-    end;
-    introduce EFalse? c' ==> (exists (fs_r:get_Type a). a ∋ (h++lt, fs_r, ex') /\ fs_beh fs_ex h lt fs_r) with _. begin
-      assert (exists (fs_r:get_Type a). a ∋ (h++lt3, fs_r, ex') /\ fs_beh fs_e h lt3 fs_r)
-    end)
+  let (c', (| lt1, (lt2, lt3) |)) = destruct_steps_eif c t e ex' h lt sts in
+  assert (qBool ∋ (h, fs_c, c') /\ lt1 == []);
+  introduce ETrue? c' ==> (exists (fs_r:get_Type a). a ∋ (h++lt, fs_r, ex') /\ fs_beh fs_ex h lt fs_r) with _. begin
+    assert (exists (fs_r:get_Type a). a ∋ (h++lt2, fs_r, ex') /\ fs_beh fs_t h lt2 fs_r)
+  end;
+  introduce EFalse? c' ==> (exists (fs_r:get_Type a). a ∋ (h++lt, fs_r, ex') /\ fs_beh fs_ex h lt fs_r) with _. begin
+    assert (exists (fs_r:get_Type a). a ∋ (h++lt3, fs_r, ex') /\ fs_beh fs_e h lt3 fs_r)
+  end)
 
 let equiv_oprod_if #g (#a:qType) (fs_c:fs_oval g qBool) (fs_t fs_e:fs_oprod g a) (c t e:exp)
   : Lemma
@@ -1180,13 +1146,10 @@ let equiv_case_prod_steps_pre (e e':closed_exp) (h:history) (lt:local_trace h) (
   ((b ^->!@ c) ⦂ (h, fs_inrc, ELam inrc))
 
 let equiv_case_prod_steps #e #e' #h #lt #a #b #c #fs_cond #fs_inlc #fs_inrc #fs_e #cond #inlc #inrc (sq:squash (equiv_case_prod_steps_pre e e' h lt a b c fs_cond fs_inlc fs_inrc fs_e cond inlc inrc)) : squash (exists (fs_r:get_Type c). c ∋ (h++lt, fs_r, e') /\ fs_beh fs_e h lt fs_r) =
-  exp_type_history_independence (a ^+ b) h fs_cond cond;
-  safety_val #(a ^+ b) fs_cond cond;
-  sem_expr_shape_val #(a ^+ b) fs_cond cond h;
-  let a_typ = type_quotation_to_typ (get_rel a) in
-  let b_typ = type_quotation_to_typ (get_rel b) in
+  lem_forall_values_are_values (a ^+ b) h fs_cond;
+  assert (forall cond' lt'. steps cond cond' h lt' /\ indexed_irred cond' (h++lt') ==> ((EInl? cond' \/ EInr? cond') /\ is_value cond'));
   FStar.Squash.bind_squash #(steps e e' h lt) () (fun sts ->
-    let (cond', (| lt1, (lt2, lt3) |)) = destruct_steps_ecase cond inlc inrc e' h lt sts a_typ b_typ in
+    let (cond', (| lt1, (lt2, lt3) |)) = destruct_steps_ecase cond inlc inrc e' h lt sts in
     match cond' with
     | EInl c' -> begin
       assert (steps (ELam inlc) (ELam inlc) h []);
@@ -1249,4 +1212,4 @@ let equiv_oprod_case #g (#a #b #c:qType) (fs_cond:fs_oval g (a ^+ b)) (fs_inlc:f
       end
     end
   end
-#pop-options*)
+#pop-options
